$$\tag{可逆过程的表达式}TdS=dE+\bar{d}A$$

## 推导过程 

$$\begin{eqnarray}
&&\oint_{(1)}^{(2)} \frac{\bar{d}Q}{T} \overset{Def}{=} S_{2}-S_{1}= \triangle S\\
&对于\underline{\textbf{可逆的元过程}}& \qquad dS=\frac{\bar{d}Q}{T}\\
&因此& \qquad TdS=\bar{d}Q\\
&热力学第一定律得到& \qquad \bar{d}Q=dE+\bar{d}A\\
&也就是说& \qquad TdS=dE+\bar{d}A
\end{eqnarray}$$


> [!attention] **特别地**
> $$对于\underline{\textbf{等熵过程}} \qquad dS=0$$


> [!summary] **注意点**
> 只适用于**<font color="#f79646">可逆</font>**过程
> $$\begin{eqnarray}
> &①& \quad \triangle S =S_{2} - S_{1} =\int^{2}_{1} \frac{\bar{d}Q}{T}\\
> &②& \quad dS= \frac{\bar{d}Q}{T}
\end{eqnarray}$$