![[Pasted image 20240402170646.png]]

$$由于 \qquad W = q \phi_{+} + (-q) \phi_{-}\quad (选取O为电势零点)$$
$$\begin{eqnarray}
因此 \qquad 
W
&=&
q \int^{(0)}_{+} \overrightarrow{E } \cdot d \overrightarrow{l} + (-q) \int^{(0)}_{-} \overrightarrow{E } \cdot d \overrightarrow{l}\\
&=&
q \int^{-}_{+} \overrightarrow{E} \cdot d \overrightarrow{l} \quad \left(\ \ q \cdot \left(-\overrightarrow{E} \cdot \frac{l}{2} \cos \theta\right)+ (-q) \cdot (\overrightarrow{E} \cdot \frac{l}{2} \cos \theta)\ \ \right)\\
&=&
- q \overrightarrow{l} \cdot \overrightarrow{E}\\
&=&
- \overrightarrow{p} \cdot \overrightarrow{E}
\end{eqnarray}$$

因此
$$E=\left\{\begin{matrix}
 \theta=0 \quad W=-pE \quad 能量\underline{\textbf{最低}}\\   \theta=\frac{\pi}{2} \quad W=0 \quad 平衡位置
 \\\theta=\pi \quad W=pE \quad 能量\underline{\textbf{最高}}

\end{matrix}\right.$$
